Cook_Levin/IMP-_To_SAS+/IMP-_To_IMP--/IMP_Minus_To_IMP_Minus_Minus_IMP.thy
@@ -1,0 +1,572 @@
+\<^marker>\<open>creator Alexander Taepper\<close>
+
+theory IMP_Minus_To_IMP_Minus_Minus_IMP
+  imports
+    Primitives_IMP_Minus
+    Binary_Arithmetic_IMP
+    IMP_Minus_To_IMP_Minus_Minus_State_Translations_IMP
+    IMP_Minus_To_IMP_Minus_Minus_nat
+    IMP_Minus.Com
+begin
+
+
+unbundle IMP_Minus_Minus_Com.no_com_syntax
+
+
+subsection \<open>Useful Definitions and Lemmas\<close>
+
+
+subsection \<open>map_var_bit_to_var\<close>
+
+subsubsection \<open>map_var_bit_to_var_acc\<close>
+
+fun map_var_bit_to_var_acc' :: "nat \<Rightarrow> nat \<Rightarrow> nat \<Rightarrow> nat" where 
+"map_var_bit_to_var_acc' acc v n = (if n \<noteq> 0 
+   then (map_var_bit_to_var_acc' ((var_bit_to_var_nat (prod_encode (v,hd_nat n)))## acc) v (tl_nat n))
+   else acc)"
+
+lemma "map_var_bit_to_var_acc' acc v n = map_var_bit_to_var_acc acc v n"
+proof (induction n arbitrary: acc v rule: less_induct)
+  case (less x)
+  then show ?case
+  proof(cases x)
+    case (Suc nat)
+    have "tl_nat x < x" using Suc
+      by simp
+    then show ?thesis
+      using less by force
+  qed (simp)
+qed
+
+record map_var_bit_to_var_acc_state =
+  map_var_bit_to_var_acc_acc::nat
+  map_var_bit_to_var_acc_v::nat
+  map_var_bit_to_var_acc_n::nat
+  map_var_bit_to_var_acc_ret::nat
+
+abbreviation "map_var_bit_to_var_acc_prefix \<equiv> ''map_var_bit_to_var_acc.''"
+abbreviation "map_var_bit_to_var_acc_acc_str \<equiv> ''acc''"
+abbreviation "map_var_bit_to_var_acc_v_str \<equiv> ''v''"
+abbreviation "map_var_bit_to_var_acc_n_str \<equiv> ''n''"
+abbreviation "map_var_bit_to_var_acc_ret_str \<equiv> ''ret''"
+
+definition "map_var_bit_to_var_acc_state_upd s \<equiv>
+  let
+    hd_xs' = map_var_bit_to_var_acc_n s;
+    hd_ret' = 0;
+    hd_state = \<lparr>hd_xs = hd_xs',
+                hd_ret = hd_ret'\<rparr>;
+    hd_ret_state = hd_imp hd_state;
+    hd_result = hd_ret hd_ret_state;
+    prod_encode_a' = map_var_bit_to_var_acc_v s;
+    prod_encode_b' = hd_result;
+    prod_encode_ret' = 0;
+    prod_encode_state = \<lparr>prod_encode_a = prod_encode_a',
+                         prod_encode_b = prod_encode_b',
+      prod_encode_ret = prod_encode_ret'\<rparr>;
+    prod_encode_ret_state = prod_encode_imp prod_encode_state;
+    prod_encode_result = prod_encode_ret prod_encode_ret_state;
+    var_bit_to_var_nat_n' = prod_encode_result;
+    var_bit_to_var_nat_ret' = 0;
+    var_bit_to_var_nat_state = \<lparr>var_bit_to_var_nat_n = var_bit_to_var_nat_n',
+                                var_bit_to_var_nat_ret = var_bit_to_var_nat_ret'\<rparr>;
+    var_bit_to_var_nat_ret_state = var_bit_to_var_nat_imp var_bit_to_var_nat_state;
+    var_bit_to_var_nat_result = var_bit_to_var_nat_ret var_bit_to_var_nat_ret_state;
+    cons_h' = var_bit_to_var_nat_result;
+    cons_t' = map_var_bit_to_var_acc_acc s;
+    cons_ret' = 0;
+    cons_state = \<lparr>cons_h = cons_h',
+                  cons_t = cons_t', 
+                  cons_ret = cons_ret'\<rparr>;
+    cons_ret_state = cons_imp cons_state;
+    cons_result = cons_ret cons_ret_state;
+    tl_xs' = map_var_bit_to_var_acc_n s;
+    tl_ret' = 0;
+    tl_state = \<lparr>tl_xs = tl_xs', 
+                tl_ret = tl_ret'\<rparr>;
+    tl_ret_state = tl_imp tl_state;
+    tl_result = tl_ret tl_ret_state;
+    map_var_bit_to_var_acc_acc' = cons_result;
+    map_var_bit_to_var_acc_v' = map_var_bit_to_var_acc_v s;
+    map_var_bit_to_var_acc_n' = tl_result;
+    map_var_bit_to_var_acc_ret' = map_var_bit_to_var_acc_ret s;
+    ret = \<lparr>map_var_bit_to_var_acc_acc = map_var_bit_to_var_acc_acc',
+           map_var_bit_to_var_acc_v = map_var_bit_to_var_acc_v',
+           map_var_bit_to_var_acc_n = map_var_bit_to_var_acc_n',
+           map_var_bit_to_var_acc_ret = map_var_bit_to_var_acc_ret'\<rparr>
+    in ret
+"
+
+definition "map_var_bit_to_var_acc_imp_compute_loop_condition s \<equiv>
+  (let
+    condition = map_var_bit_to_var_acc_n s
+   in condition
+  )
+"
+
+definition "map_var_bit_to_var_acc_imp_after_loop s \<equiv>
+  (let
+    map_var_bit_to_var_acc_acc' = map_var_bit_to_var_acc_acc s;
+    map_var_bit_to_var_acc_v' = map_var_bit_to_var_acc_v s;
+    map_var_bit_to_var_acc_n' = map_var_bit_to_var_acc_n s;
+    map_var_bit_to_var_acc_ret' = map_var_bit_to_var_acc_acc s;
+    ret = \<lparr>map_var_bit_to_var_acc_acc = map_var_bit_to_var_acc_acc',
+           map_var_bit_to_var_acc_v = map_var_bit_to_var_acc_v',
+           map_var_bit_to_var_acc_n = map_var_bit_to_var_acc_n',
+           map_var_bit_to_var_acc_ret = map_var_bit_to_var_acc_ret'\<rparr>
+   in ret
+  )"
+
+lemmas map_var_bit_to_var_acc_imp_subprogram_simps = 
+  map_var_bit_to_var_acc_state_upd_def
+  map_var_bit_to_var_acc_imp_compute_loop_condition_def
+  map_var_bit_to_var_acc_imp_after_loop_def
+
+function map_var_bit_to_var_acc_imp::
+  "map_var_bit_to_var_acc_state \<Rightarrow> map_var_bit_to_var_acc_state" where
+  "map_var_bit_to_var_acc_imp s =
+  (if map_var_bit_to_var_acc_imp_compute_loop_condition s \<noteq> 0
+   then
+    let next_iteration = map_var_bit_to_var_acc_imp (map_var_bit_to_var_acc_state_upd s)
+    in next_iteration
+   else
+    let ret = map_var_bit_to_var_acc_imp_after_loop s
+    in ret
+  )"
+  by simp+
+termination 
+  apply (relation "measure map_var_bit_to_var_acc_n")
+   apply (simp add: map_var_bit_to_var_acc_imp_subprogram_simps tl_imp_correct)+
+  done
+
+declare map_var_bit_to_var_acc_imp.simps [simp del]
+
+lemma map_var_bit_to_var_acc_imp_correct:
+  "map_var_bit_to_var_acc_ret (map_var_bit_to_var_acc_imp s) =
+    map_var_bit_to_var_acc' (map_var_bit_to_var_acc_acc s) 
+  (map_var_bit_to_var_acc_v s) (map_var_bit_to_var_acc_n s)"
+  apply (induction s rule: map_var_bit_to_var_acc_imp.induct)
+  apply (subst map_var_bit_to_var_acc_imp.simps)
+  apply (subst map_var_bit_to_var_acc'.simps)
+  apply (simp del: map_var_bit_to_var_acc'.simps 
+              add: map_var_bit_to_var_acc_imp_subprogram_simps Let_def 
+                   fst_nat_fst'_nat snd_nat_snd'_nat snd'_imp_correct fst'_imp_correct
+                   hd_imp_correct prod_encode_imp_correct var_bit_to_var_nat_imp_correct
+                   cons_imp_correct tl_imp_correct)
+  done            
+
+definition "map_var_bit_to_var_acc_state_upd_time t s \<equiv>
+  let
+    hd_xs' = map_var_bit_to_var_acc_n s;
+    t = t + 2;
+    hd_ret' = 0;
+    t = t + 2;
+    hd_state = \<lparr>hd_xs = hd_xs',
+                hd_ret = hd_ret'\<rparr>;
+    hd_ret_state = hd_imp hd_state;
+    t = t + hd_imp_time 0 hd_state;
+    hd_result = hd_ret hd_ret_state;
+    t = t + 2;
+    prod_encode_a' = map_var_bit_to_var_acc_v s;
+    t = t + 2;
+    prod_encode_b' = hd_result;
+    t = t + 2;
+    prod_encode_ret' = 0;
+    t = t + 2;
+    prod_encode_state = \<lparr>prod_encode_a = prod_encode_a',
+                         prod_encode_b = prod_encode_b',
+      prod_encode_ret = prod_encode_ret'\<rparr>;
+    prod_encode_ret_state = prod_encode_imp prod_encode_state;
+    t = t + prod_encode_imp_time 0 prod_encode_state;
+    prod_encode_result = prod_encode_ret prod_encode_ret_state;
+    t = t + 2;
+    var_bit_to_var_nat_n' = prod_encode_result;
+    t = t + 2;
+    var_bit_to_var_nat_ret' = 0;
+    t = t + 2;
+    var_bit_to_var_nat_state = \<lparr>var_bit_to_var_nat_n = var_bit_to_var_nat_n',
+                                var_bit_to_var_nat_ret = var_bit_to_var_nat_ret'\<rparr>;
+    var_bit_to_var_nat_ret_state = var_bit_to_var_nat_imp var_bit_to_var_nat_state;
+    t = t + var_bit_to_var_nat_imp_time 0 var_bit_to_var_nat_state;
+    var_bit_to_var_nat_result = var_bit_to_var_nat_ret var_bit_to_var_nat_ret_state;
+    t = t + 2;
+    cons_h' = var_bit_to_var_nat_result;
+    t = t + 2;
+    cons_t' = map_var_bit_to_var_acc_acc s;
+    t = t + 2;
+    cons_ret' = 0;
+    t = t + 2;
+    cons_state = \<lparr>cons_h = cons_h',
+                  cons_t = cons_t', 
+                  cons_ret = cons_ret'\<rparr>;
+    cons_ret_state = cons_imp cons_state;
+    t = t + cons_imp_time 0 cons_state;
+    cons_result = cons_ret cons_ret_state;
+    t = t + 2;
+    tl_xs' = map_var_bit_to_var_acc_n s;
+    t = t + 2;
+    tl_ret' = 0;
+    t = t + 2;
+    tl_state = \<lparr>tl_xs = tl_xs', 
+                tl_ret = tl_ret'\<rparr>;
+    tl_ret_state = tl_imp tl_state;
+    t = t + tl_imp_time 0 tl_state;
+    tl_result = tl_ret tl_ret_state;
+    t = t + 2;
+    map_var_bit_to_var_acc_acc' = cons_result;
+    t = t + 2;
+    map_var_bit_to_var_acc_v' = map_var_bit_to_var_acc_v s;
+    t = t + 2;
+    map_var_bit_to_var_acc_n' = tl_result;
+    t = t + 2;
+    map_var_bit_to_var_acc_ret' = map_var_bit_to_var_acc_ret s;
+    t = t + 2;
+    ret = \<lparr>map_var_bit_to_var_acc_acc = map_var_bit_to_var_acc_acc',
+           map_var_bit_to_var_acc_v = map_var_bit_to_var_acc_v',
+           map_var_bit_to_var_acc_n = map_var_bit_to_var_acc_n',
+           map_var_bit_to_var_acc_ret = map_var_bit_to_var_acc_ret'\<rparr>
+  in
+    t
+"
+
+definition "map_var_bit_to_var_acc_imp_compute_loop_condition_time t s \<equiv>
+  let
+    condition = map_var_bit_to_var_acc_n s;
+    t = t + 2
+  in
+    t
+"
+
+definition "map_var_bit_to_var_acc_imp_after_loop_time t s \<equiv>
+  let
+    map_var_bit_to_var_acc_acc' = map_var_bit_to_var_acc_acc s;
+    t = t + 2;
+    map_var_bit_to_var_acc_v' = map_var_bit_to_var_acc_v s;
+    t = t + 2;
+    map_var_bit_to_var_acc_n' = map_var_bit_to_var_acc_n s;
+    t = t + 2;
+    map_var_bit_to_var_acc_ret' = map_var_bit_to_var_acc_acc s;
+    t = t + 2;
+    ret = \<lparr>map_var_bit_to_var_acc_acc = map_var_bit_to_var_acc_acc',
+           map_var_bit_to_var_acc_v = map_var_bit_to_var_acc_v',
+           map_var_bit_to_var_acc_n = map_var_bit_to_var_acc_n',
+           map_var_bit_to_var_acc_ret = map_var_bit_to_var_acc_ret'\<rparr>
+  in
+    t
+"
+
+lemmas map_var_bit_to_var_acc_imp_subprogram_time_simps = 
+  map_var_bit_to_var_acc_state_upd_time_def
+  map_var_bit_to_var_acc_imp_compute_loop_condition_time_def
+  map_var_bit_to_var_acc_imp_after_loop_time_def
+  map_var_bit_to_var_acc_imp_subprogram_simps
+
+function map_var_bit_to_var_acc_imp_time::
+  "nat \<Rightarrow> map_var_bit_to_var_acc_state \<Rightarrow> nat" where
+  "map_var_bit_to_var_acc_imp_time t s =
+  map_var_bit_to_var_acc_imp_compute_loop_condition_time 0 s +
+  (if map_var_bit_to_var_acc_imp_compute_loop_condition s \<noteq> 0
+    then
+      (let
+        t = t + 1;
+        next_iteration =
+          map_var_bit_to_var_acc_imp_time (t + map_var_bit_to_var_acc_state_upd_time 0 s)
+                         (map_var_bit_to_var_acc_state_upd s)
+       in next_iteration)
+    else
+      (let
+        t = t + 2;
+        ret = t + map_var_bit_to_var_acc_imp_after_loop_time 0 s
+       in ret)
+  )"
+  by auto
+termination
+  apply (relation "measure (map_var_bit_to_var_acc_n \<circ> snd)")
+  by (auto simp add: map_var_bit_to_var_acc_imp_subprogram_time_simps tl_imp_correct)
+
+declare map_var_bit_to_var_acc_imp_time.simps [simp del]            
+
+lemma map_var_bit_to_var_acc_imp_time_acc:
+  "(map_var_bit_to_var_acc_imp_time (Suc t) s) = Suc (map_var_bit_to_var_acc_imp_time t s)"
+  by (induction t s rule: map_var_bit_to_var_acc_imp_time.induct)
+    ((subst (1 2) map_var_bit_to_var_acc_imp_time.simps);
+      (simp add: map_var_bit_to_var_acc_state_upd_def))            
+
+lemma map_var_bit_to_var_acc_imp_time_acc_2_aux:
+  "(map_var_bit_to_var_acc_imp_time t s) = t + (map_var_bit_to_var_acc_imp_time 0 s)"
+  by (induction t arbitrary: s) (simp add: map_var_bit_to_var_acc_imp_time_acc)+            
+
+lemma map_var_bit_to_var_acc_imp_time_acc_2:
+  "t \<noteq> 0 \<Longrightarrow> (map_var_bit_to_var_acc_imp_time t s) = t + (map_var_bit_to_var_acc_imp_time 0 s)"
+  by (rule map_var_bit_to_var_acc_imp_time_acc_2_aux)            
+
+lemma map_var_bit_to_var_acc_imp_time_acc_3:
+  "(map_var_bit_to_var_acc_imp_time (a + b) s) = a + (map_var_bit_to_var_acc_imp_time b s)"
+  by (induction a arbitrary: b s) (simp add: map_var_bit_to_var_acc_imp_time_acc)+            
+
+abbreviation "map_var_bit_to_var_acc_while_cond \<equiv> ''condition''"
+abbreviation "map_var_bit_to_var_acc_hd_result \<equiv> ''hd_result''"
+abbreviation "map_var_bit_to_var_acc_prod_encode_result \<equiv> ''prod_encode_result''"
+abbreviation "map_var_bit_to_var_acc_var_bit_to_var_nat_result \<equiv> ''var_bit_to_var_nat_result''"
+abbreviation "map_var_bit_to_var_acc_cons_result \<equiv> ''cons_result''"
+abbreviation "map_var_bit_to_var_acc_tl_result \<equiv> ''tl_result''"
+
+definition "map_var_bit_to_var_acc_IMP_init_while_cond \<equiv>
+  \<comment> \<open>condition = map_var_bit_to_var_acc_n s\<close>
+  map_var_bit_to_var_acc_while_cond ::= A (V map_var_bit_to_var_acc_n_str)
+"
+
+definition "map_var_bit_to_var_acc_IMP_loop_body \<equiv>
+  \<comment> \<open>hd_xs' = map_var_bit_to_var_acc_n s;\<close>
+  (hd_prefix @ hd_xs_str) ::= (A (V map_var_bit_to_var_acc_n_str));;
+  \<comment> \<open>hd_ret' = 0;\<close>
+  (hd_prefix @ hd_ret_str) ::= (A (N 0));;
+  \<comment> \<open>hd_state = \<lparr>hd_xs = hd_xs',\<close>
+  \<comment> \<open>            hd_ret = hd_ret'\<rparr>;\<close>
+  \<comment> \<open>hd_ret_state = hd_imp hd_state;\<close>
+  invoke_subprogram hd_prefix hd_IMP_Minus;;
+  \<comment> \<open>hd_result = hd_ret hd_ret_state;\<close>
+  map_var_bit_to_var_acc_hd_result ::= (A (V (hd_prefix @ hd_ret_str)));;
+  \<comment> \<open>prod_encode_a' = map_var_bit_to_var_acc_v s;\<close>
+  (prod_encode_prefix @ prod_encode_a_str) ::= (A (V map_var_bit_to_var_acc_v_str));;
+  \<comment> \<open>prod_encode_b' = hd_result;\<close>
+  (prod_encode_prefix @ prod_encode_b_str) ::= (A (V map_var_bit_to_var_acc_hd_result));;
+  \<comment> \<open>prod_encode_ret' = 0;\<close>
+  (prod_encode_prefix @ prod_encode_ret_str) ::= (A (N 0));;
+  \<comment> \<open>prod_encode_state = \<lparr>prod_encode_a = prod_encode_a',\<close>
+  \<comment> \<open>                     prod_encode_b = prod_encode_b',\<close>
+  \<comment> \<open>  prod_encode_ret = prod_encode_ret'\<rparr>;\<close>
+  \<comment> \<open>prod_encode_ret_state = prod_encode_imp prod_encode_state;\<close>
+  invoke_subprogram prod_encode_prefix prod_encode_IMP_Minus;;
+  \<comment> \<open>prod_encode_result = prod_encode_ret prod_encode_ret_state;\<close>
+  map_var_bit_to_var_acc_prod_encode_result ::= (A (V (prod_encode_prefix @ prod_encode_ret_str)));;
+  \<comment> \<open>var_bit_to_var_nat_n' = prod_encode_result;\<close>
+  (var_bit_to_var_nat_prefix @ var_bit_to_var_nat_n_str) ::= (A (V map_var_bit_to_var_acc_prod_encode_result));;
+  \<comment> \<open>var_bit_to_var_nat_ret' = 0;\<close>
+  (var_bit_to_var_nat_prefix @ var_bit_to_var_nat_ret_str) ::= (A (N 0));;
+  \<comment> \<open>var_bit_to_var_nat_state = \<lparr>var_bit_to_var_nat_n = var_bit_to_var_nat_n',\<close>
+  \<comment> \<open>                            var_bit_to_var_nat_ret = var_bit_to_var_nat_ret'\<rparr>;\<close>
+  \<comment> \<open>var_bit_to_var_nat_ret_state = var_bit_to_var_nat_imp var_bit_to_var_nat_state;\<close>
+  invoke_subprogram var_bit_to_var_nat_prefix var_bit_to_var_nat_IMP_Minus;;
+  \<comment> \<open>var_bit_to_var_nat_result = var_bit_to_var_nat_ret var_bit_to_var_nat_ret_state;\<close>
+  map_var_bit_to_var_acc_var_bit_to_var_nat_result ::= (A (V (var_bit_to_var_nat_prefix @ var_bit_to_var_nat_ret_str)));;
+  \<comment> \<open>cons_h' = var_bit_to_var_nat_result;\<close>
+  (cons_prefix @ cons_h_str) ::= (A (V map_var_bit_to_var_acc_var_bit_to_var_nat_result));;
+  \<comment> \<open>cons_t' = map_var_bit_to_var_acc_acc s;\<close>
+  (cons_prefix @ cons_t_str) ::= (A (V map_var_bit_to_var_acc_acc_str));;
+  \<comment> \<open>cons_ret' = 0;\<close>
+  (cons_prefix @ cons_ret_str) ::= (A (N 0));;
+  \<comment> \<open>cons_state = \<lparr>cons_h = cons_h',\<close>
+  \<comment> \<open>              cons_t = cons_t', \<close>
+  \<comment> \<open>              cons_ret = cons_ret'\<rparr>;\<close>
+  \<comment> \<open>cons_ret_state = cons_imp cons_state;\<close>
+  invoke_subprogram cons_prefix cons_IMP_Minus;;
+  \<comment> \<open>cons_result = cons_ret cons_ret_state;\<close>
+  map_var_bit_to_var_acc_cons_result ::= (A (V (cons_prefix @ cons_ret_str)));;
+  \<comment> \<open>tl_xs' = map_var_bit_to_var_acc_n s;\<close>
+  (tl_prefix @ tl_xs_str) ::= (A (V map_var_bit_to_var_acc_n_str));;
+  \<comment> \<open>tl_ret' = 0;\<close>
+  (tl_prefix @ tl_ret_str) ::= (A (N 0));;
+  \<comment> \<open>tl_state = \<lparr>tl_xs = tl_xs', \<close>
+  \<comment> \<open>            tl_ret = tl_ret'\<rparr>;\<close>
+  \<comment> \<open>tl_ret_state = tl_imp tl_state;\<close>
+  invoke_subprogram tl_prefix tl_IMP_Minus;;
+  \<comment> \<open>tl_result = tl_ret tl_ret_state;\<close>
+  map_var_bit_to_var_acc_tl_result ::= (A (V (tl_prefix @ tl_ret_str)));;
+  \<comment> \<open>map_var_bit_to_var_acc_acc' = cons_result;\<close>
+  (map_var_bit_to_var_acc_acc_str) ::= (A (V map_var_bit_to_var_acc_cons_result));;
+  \<comment> \<open>map_var_bit_to_var_acc_v' = map_var_bit_to_var_acc_v s;\<close>
+  (map_var_bit_to_var_acc_v_str) ::= (A (V map_var_bit_to_var_acc_v_str));;
+  \<comment> \<open>map_var_bit_to_var_acc_n' = tl_result;\<close>
+  (map_var_bit_to_var_acc_n_str) ::= (A (V map_var_bit_to_var_acc_tl_result));;
+  \<comment> \<open>map_var_bit_to_var_acc_ret' = map_var_bit_to_var_acc_ret s;\<close>
+  (map_var_bit_to_var_acc_ret_str) ::= (A (V map_var_bit_to_var_acc_ret_str))
+  \<comment> \<open>ret = \<lparr>map_var_bit_to_var_acc_acc = map_var_bit_to_var_acc_acc',\<close>
+  \<comment> \<open>       map_var_bit_to_var_acc_v = map_var_bit_to_var_acc_v',\<close>
+  \<comment> \<open>       map_var_bit_to_var_acc_n = map_var_bit_to_var_acc_n',\<close>
+  \<comment> \<open>       map_var_bit_to_var_acc_ret = map_var_bit_to_var_acc_ret'\<rparr>\<close>
+"
+
+definition "map_var_bit_to_var_acc_IMP_after_loop \<equiv>
+  \<comment> \<open>map_var_bit_to_var_acc_acc' = map_var_bit_to_var_acc_acc s;\<close>
+  (map_var_bit_to_var_acc_acc_str) ::= (A (V map_var_bit_to_var_acc_cons_result));;
+  \<comment> \<open>map_var_bit_to_var_acc_v' = map_var_bit_to_var_acc_v s;\<close>
+  (map_var_bit_to_var_acc_v_str) ::= (A (V map_var_bit_to_var_acc_v_str));;
+  \<comment> \<open>map_var_bit_to_var_acc_n' = map_var_bit_to_var_acc_n s;\<close>
+  (map_var_bit_to_var_acc_n_str) ::= (A (V map_var_bit_to_var_acc_tl_result));;
+  \<comment> \<open>map_var_bit_to_var_acc_ret' = map_var_bit_to_var_acc_acc s;\<close>
+  (map_var_bit_to_var_acc_ret_str) ::= (A (V map_var_bit_to_var_acc_cons_result))
+  \<comment> \<open>ret = \<lparr>map_var_bit_to_var_acc_acc = map_var_bit_to_var_acc_acc',\<close>
+  \<comment> \<open>       map_var_bit_to_var_acc_v = map_var_bit_to_var_acc_v',\<close>
+  \<comment> \<open>       map_var_bit_to_var_acc_n = map_var_bit_to_var_acc_n',\<close>
+  \<comment> \<open>       map_var_bit_to_var_acc_ret = map_var_bit_to_var_acc_ret'\<rparr>\<close>
+"
+
+definition map_var_bit_to_var_acc_IMP_Minus where
+  "map_var_bit_to_var_acc_IMP_Minus \<equiv>
+  map_var_bit_to_var_acc_IMP_init_while_cond;;
+  WHILE map_var_bit_to_var_acc_while_cond \<noteq>0 DO (
+    map_var_bit_to_var_acc_IMP_loop_body;;
+    map_var_bit_to_var_acc_IMP_init_while_cond
+  );;
+  map_var_bit_to_var_acc_IMP_after_loop"
+
+abbreviation "map_var_bit_to_var_acc_IMP_vars\<equiv>
+  {map_var_bit_to_var_acc_while_cond, map_var_bit_to_var_acc_hd_result,
+    map_var_bit_to_var_acc_prod_encode_result, map_var_bit_to_var_acc_var_bit_to_var_nat_result,
+    map_var_bit_to_var_acc_cons_result, map_var_bit_to_var_acc_tl_result}"
+
+lemmas map_var_bit_to_var_acc_IMP_subprogram_simps =
+  map_var_bit_to_var_acc_IMP_init_while_cond_def
+  map_var_bit_to_var_acc_IMP_loop_body_def
+  map_var_bit_to_var_acc_IMP_after_loop_def
+
+definition "map_var_bit_to_var_acc_imp_to_HOL_state p s =
+  \<lparr>map_var_bit_to_var_acc_acc = (s (add_prefix p map_var_bit_to_var_acc_acc_str)),
+  map_var_bit_to_var_acc_v = (s (add_prefix p map_var_bit_to_var_acc_v_str)),
+  map_var_bit_to_var_acc_n = (s (add_prefix p map_var_bit_to_var_acc_n_str)),
+  map_var_bit_to_var_acc_ret = (s (add_prefix p map_var_bit_to_var_acc_ret_str))\<rparr>"
+
+lemmas map_var_bit_to_var_acc_state_translators =
+  map_var_bit_to_var_acc_imp_to_HOL_state_def
+  hd_imp_to_HOL_state_def
+  prod_encode_imp_to_HOL_state_def
+  var_bit_to_var_nat_imp_to_HOL_state_def
+  cons_imp_to_HOL_state_def
+  tl_imp_to_HOL_state_def
+
+lemmas map_var_bit_to_var_acc_complete_simps =
+  map_var_bit_to_var_acc_IMP_subprogram_simps
+  map_var_bit_to_var_acc_imp_subprogram_simps
+  map_var_bit_to_var_acc_state_translators
+
+lemma map_var_bit_to_var_acc_IMP_Minus_correct_function:
+  "(invoke_subprogram p map_var_bit_to_var_acc_IMP_Minus, s) \<Rightarrow>\<^bsup>t\<^esup> s' \<Longrightarrow>
+     s' (add_prefix p map_var_bit_to_var_acc_ret_str)
+      = map_var_bit_to_var_acc_ret
+          (map_var_bit_to_var_acc_imp (map_var_bit_to_var_acc_imp_to_HOL_state p s))"
+  apply(induction "map_var_bit_to_var_acc_imp_to_HOL_state p s" arbitrary: s s' t
+    rule: map_var_bit_to_var_acc_imp.induct)
+  apply(subst map_var_bit_to_var_acc_imp.simps)
+  apply(simp only: map_var_bit_to_var_acc_IMP_Minus_def prefix_simps)
+  apply(erule Seq_E)+
+  apply(erule While_tE)
+
+  subgoal
+    apply(simp only: map_var_bit_to_var_acc_IMP_subprogram_simps prefix_simps)
+    apply(erule Seq_E)+
+    apply(fastforce_sorted_premises2 simp: map_var_bit_to_var_acc_IMP_subprogram_simps
+        map_var_bit_to_var_acc_imp_subprogram_simps
+        map_var_bit_to_var_acc_state_translators)
+
+  apply(erule Seq_E)+
+  apply(dest_com_gen)
+
+  subgoal
+      apply(simp only: map_var_bit_to_var_acc_IMP_init_while_cond_def prefix_simps)
+      apply(erule Seq_E)+
+      apply(erule <?>_IMP_Minus_correct[where vars = "map_var_bit_to_var_acc_IMP_vars"])
+      subgoal premises p using p(999) by fastforce
+      by(fastforce simp add: map_var_bit_to_var_acc_complete_simps)
+
+  subgoal
+      apply(subst (asm) map_var_bit_to_var_acc_IMP_init_while_cond_def)
+      apply(simp only: map_var_bit_to_var_acc_IMP_loop_body_def prefix_simps)
+      apply(erule Seq_E)+
+      apply(erule <?>_IMP_Minus_correct[where vars = "map_var_bit_to_var_acc_IMP_vars"])
+      subgoal premises p using p(999) by fastforce
+      by (simp only: map_var_bit_to_var_acc_imp_subprogram_simps
+          map_var_bit_to_var_acc_state_translators Let_def, force)
+
+  subgoal
+      apply(simp only: map_var_bit_to_var_acc_IMP_init_while_cond_def prefix_simps
+          map_var_bit_to_var_acc_IMP_loop_body_def)
+      apply(erule Seq_E)+
+      apply(erule <?>_IMP_Minus_correct[where vars = "map_var_bit_to_var_acc_IMP_vars"])
+      subgoal premises p using p(999) by fastforce
+      by (simp only: map_var_bit_to_var_acc_imp_subprogram_simps
+          map_var_bit_to_var_acc_state_translators Let_def, force)
+  done        
+
+lemma map_var_bit_to_var_acc_IMP_Minus_correct_effects:
+  "\<lbrakk>(invoke_subprogram (p @ map_var_bit_to_var_acc_pref) map_var_bit_to_var_acc_IMP_Minus, s) \<Rightarrow>\<^bsup>t\<^esup> s';
+    v \<in> vars; \<not> (prefix map_var_bit_to_var_acc_pref v)\<rbrakk>
+   \<Longrightarrow> s (add_prefix p v) = s' (add_prefix p v)"
+  using com_add_prefix_valid'' com_only_vars prefix_def
+  by blast            
+
+lemmas map_var_bit_to_var_acc_complete_time_simps =
+  map_var_bit_to_var_acc_imp_subprogram_time_simps
+  map_var_bit_to_var_acc_imp_time_acc
+  map_var_bit_to_var_acc_imp_time_acc_2
+  map_var_bit_to_var_acc_imp_time_acc_3
+  map_var_bit_to_var_acc_state_translators
+
+lemma map_var_bit_to_var_acc_IMP_Minus_correct_time:
+  "(invoke_subprogram p map_var_bit_to_var_acc_IMP_Minus, s) \<Rightarrow>\<^bsup>t\<^esup> s' \<Longrightarrow>
+     t = map_var_bit_to_var_acc_imp_time 0 (map_var_bit_to_var_acc_imp_to_HOL_state p s)"
+  apply(induction "map_var_bit_to_var_acc_imp_to_HOL_state p s" arbitrary: s s' t
+      rule: map_var_bit_to_var_acc_imp.induct)
+  apply(subst map_var_bit_to_var_acc_imp_time.simps)
+  apply(simp only: map_var_bit_to_var_acc_IMP_Minus_def prefix_simps)
+
+  apply(erule Seq_tE)+
+  apply(erule While_tE_time)
+
+  subgoal
+    apply(simp only: map_var_bit_to_var_acc_IMP_subprogram_simps prefix_simps)
+    apply(erule Seq_tE)+
+    apply(erule <?>_IMP_Minus_correct[where vars = "map_var_bit_to_var_acc_IMP_vars"])
+    subgoal premises p using p(999) by fastforce
+    by (force simp: map_var_bit_to_var_acc_IMP_subprogram_simps
+        map_var_bit_to_var_acc_imp_subprogram_time_simps map_var_bit_to_var_acc_state_translators)
+
+  apply(erule Seq_tE)+
+  apply(simp add: add.assoc)
+  apply(dest_com_gen_time)
+
+  subgoal
+    apply(simp only: map_var_bit_to_var_acc_IMP_init_while_cond_def prefix_simps)
+    apply(erule Seq_tE)+
+    apply(erule <?>_IMP_Minus_correct[where vars = "map_var_bit_to_var_acc_IMP_vars"])
+    subgoal premises p using p(999) by fastforce
+    by(fastforce simp add: map_var_bit_to_var_acc_complete_simps)
+
+  subgoal
+    apply(subst (asm) map_var_bit_to_var_acc_IMP_init_while_cond_def)
+    apply(simp only: map_var_bit_to_var_acc_IMP_loop_body_def prefix_simps)
+    apply(erule Seq_tE)+
+    apply(erule <?>_IMP_Minus_correct[where vars = "map_var_bit_to_var_acc_IMP_vars"])
+    subgoal premises p using p(999) by fastforce
+    by (simp only: map_var_bit_to_var_acc_imp_subprogram_time_simps
+        map_var_bit_to_var_acc_state_translators Let_def, force)
+
+  subgoal
+    apply(simp only: prefix_simps map_var_bit_to_var_acc_IMP_init_while_cond_def
+        map_var_bit_to_var_acc_IMP_loop_body_def)
+    apply(erule Seq_tE)+
+    apply(erule <?>_IMP_Minus_correct[where vars = "map_var_bit_to_var_acc_IMP_vars"])
+    subgoal premises p using p(999) by fastforce
+    apply(simp only: map_var_bit_to_var_acc_complete_time_simps Let_def)
+    by force
+
+  done        
+
+lemma map_var_bit_to_var_acc_IMP_Minus_correct:
+  "\<lbrakk>(invoke_subprogram (p1 @ p2) map_var_bit_to_var_acc_IMP_Minus, s) \<Rightarrow>\<^bsup>t\<^esup> s';
+    \<And>v. v \<in> vars \<Longrightarrow> \<not> (set p2 \<subseteq> set v);
+    \<lbrakk>t = (map_var_bit_to_var_acc_imp_time 0 (map_var_bit_to_var_acc_imp_to_HOL_state (p1 @ p2) s));
+     s' (add_prefix (p1 @ p2) map_var_bit_to_var_acc_ret_str) =
+          map_var_bit_to_var_acc_ret (map_var_bit_to_var_acc_imp
+                                        (map_var_bit_to_var_acc_imp_to_HOL_state (p1 @ p2) s));
+     \<And>v. v \<in> vars \<Longrightarrow> s (add_prefix p1 v) = s' (add_prefix p1 v)\<rbrakk>
+   \<Longrightarrow> P\<rbrakk> \<Longrightarrow> P"
+  using map_var_bit_to_var_acc_IMP_Minus_correct_function
+  by (auto simp: map_var_bit_to_var_acc_IMP_Minus_correct_time)
+    (meson map_var_bit_to_var_acc_IMP_Minus_correct_effects set_mono_prefix) 
+
+subsubsection \<open>map_var_bit_to_var_tail\<close>
+
+
+
+end
